Hw12 submitted

sf/Assignment12_05.v
@@ -13,31 +13,53 @@ Require Export Assignment12_04.
 *)
 
 Definition halve : tm :=
-  FILL_IN_HERE.
+  tfix
+    (tabs Halve (TArrow TNat TNat)
+      (tabs X TNat
+        (tif0
+          (tvar X)
+          (tnat 0)
+          (tif0
+            (tpred (tvar X))
+            (tnat 0)
+            (tsucc (tapp (tvar Halve) (tpred (tpred (tvar X))))))))).
 
 Example halve_type: empty |- halve \in TArrow TNat TNat.
 Proof.
+unfold halve; eauto 10.
   (* unfold halve; eauto 10. *)
-  exact FILL_IN_HERE.
 Qed.
 
 Example halve_10: tapp halve (tnat 10) ==>* tnat 5.
 Proof.
-  (* unfold halve; normalize. *)
-  exact FILL_IN_HERE.
+unfold halve; normalize.
 Qed.
 
 Example halve_11: tapp halve (tnat 11) ==>* tnat 5.
 Proof.
-  (* unfold halve; normalize. *)
-  exact FILL_IN_HERE.
+unfold halve; normalize.
 Qed.
 
 
 Theorem halve_correct: forall n,
    tapp halve (tnat (n+n)) ==>* tnat n.
 Proof.
-  exact FILL_IN_HERE.
+intros. induction n. unfold halve. normalize.
+eapply multi_step. apply ST_AppFix. constructor. constructor.
+eapply multi_step. apply ST_App1. apply ST_AppAbs. constructor. constructor. simpl.
+eapply multi_step. apply ST_AppAbs. constructor. simpl. 
+eapply multi_step. apply ST_If0Nonzero.
+eapply multi_step. apply ST_If01. apply ST_PredNat. simpl. rewrite <- plus_comm. simpl.
+eapply multi_step. apply ST_If0Nonzero.
+eapply multi_step. apply ST_Succ1. apply ST_App2. constructor. constructor. apply ST_Pred. apply ST_PredNat.
+eapply multi_step. apply ST_Succ1. apply ST_App2. constructor. constructor. apply ST_PredNat. simpl.
+inversion IHn. subst.
+eapply multi_step. apply ST_Succ1. apply H.
+apply multi_trans with (y:= tsucc (tnat n)).
+assert (forall a b, (multi step a b) -> (multi step (tsucc a) (tsucc b))).
+{ intros. induction H1. constructor. eapply multi_step. constructor. apply H1. apply IHmulti. }
+apply H1. apply H0.
+apply multi_step with (y0:= (tnat (S n))). constructor. constructor.
 Qed.
 
 (*-- Check --*)
