sf/Assignment12_01.v
@@ -15,7 +15,12 @@ Example typing_nonexample_3 :
              (tapp (tvar X) (tvar X))) \in
           T).
 Proof.
-  exact FILL_IN_HERE.
+unfold not. intros. destruct H. destruct H; subst.
+inversion H; subst. inversion H5; subst. inversion H3; subst. inversion H6; subst. rewrite H2 in H4.
+inversion H4. rewrite H1 in *. clear H6. clear H4.
+remember T1. induction t; try inversion H1.
+rewrite H6 in *. clear H6. apply IHt1. rewrite <- Heqt. symmetry. assumption.
+rewrite H4 in H3. assumption. rewrite H4 in H2. assumption. assumption.
 Qed.
 
 (*-- Check --*)
