sf/Assignment12_02.v
@@ -7,7 +7,9 @@ Corollary typable_empty__closed : forall t T,
     empty |- t \in T  ->
     closed t.
 Proof.
-  exact FILL_IN_HERE.
+unfold closed. unfold not. intros.
+apply free_in_context with (Gamma:=empty) (T:=T) in H0.
+inversion H0. inversion H1. apply H. 
 Qed.
 
 (*-- Check --*)
