sf/Assignment12_03.v
@@ -12,7 +12,28 @@ Lemma type_is_unique: forall t G T T'
     (TYPED': G |- t \in T'),
   T = T'.
 Proof.
-  exact FILL_IN_HERE.
+intros. generalize dependent T'.
+induction TYPED; subst.
+intros. inversion TYPED'. rewrite H in H2. inversion H2; reflexivity.
+intros. inversion TYPED'; subst. apply IHTYPED in H4. rewrite H4. reflexivity.
+intros. inversion TYPED'; subst. apply IHTYPED1 in H2. apply IHTYPED2 in H4. subst. inversion H2. reflexivity.
+intros. inversion TYPED'; subst. reflexivity.
+intros. inversion TYPED'; subst. reflexivity.
+intros. inversion TYPED'; subst. reflexivity.
+intros. inversion TYPED'; subst. reflexivity.
+intros. inversion TYPED'; subst. apply IHTYPED2 in H5. assumption.
+intros. inversion TYPED'; subst. apply IHTYPED1 in H2. apply IHTYPED2 in H4. subst. reflexivity.
+intros. inversion TYPED'; subst. apply IHTYPED in H1. inversion H1. reflexivity.
+intros. inversion TYPED'; subst. apply IHTYPED in H1. inversion H1. reflexivity.
+intros. inversion TYPED'; subst. reflexivity.
+intros. inversion TYPED'; subst. apply IHTYPED1 in H4. subst. apply IHTYPED2 in H5. assumption.
+intros. inversion TYPED'; subst. apply IHTYPED in H3. subst. reflexivity.
+intros. inversion TYPED'; subst. apply IHTYPED in H3. subst. reflexivity.
+intros. inversion TYPED'; subst. apply IHTYPED1 in H6. inversion H6. subst. apply IHTYPED2 in H7. assumption.
+intros. inversion TYPED'; subst. reflexivity.
+intros. inversion TYPED'; subst. apply IHTYPED1 in H2. subst. reflexivity.
+intros. inversion TYPED'; subst. apply IHTYPED1 in H6. inversion H6. subst. apply IHTYPED2 in H7. assumption.
+intros. inversion TYPED'; subst. apply IHTYPED in H1. inversion H1. reflexivity.
 Qed.
 
 (*-- Check --*)
