sf/Assignment12_06.v
@@ -5,7 +5,68 @@ Require Export Assignment12_05.
 Theorem tloop_diverges:
   ~ exists t, tapp tloop (tnat 0) ==>* t /\ normal_form step t.
 Proof.
-  exact FILL_IN_HERE.
+assert (K: exists Q R, tapp tloop (tnat 0) ==> Q /\ Q ==> R /\ R ==> tapp tloop (tnat 0)).
+{ eapply ex_intro. eapply ex_intro. split. unfold tloop. auto. split. auto. simpl. unfold tloop. apply ST_AppAbs. trivial. }
+
+assert (K0: forall v, value v -> (exists v', v ==> v') -> False).
+{ intros. induction v; try (inversion H); subst; inversion H0; subst; try inversion H1; eauto. }
+
+assert (K1: deterministic step).
+{ unfold deterministic. intros. generalize dependent y2. induction H; intros.
+  inversion H0. auto. solve by inversion.
+  subst. exfalso. apply K0 with v2. auto. exists t2'. auto.
+  inversion H0. eauto. solve by inversion 2. apply IHstep in H4. subst. auto.
+  subst. exfalso. apply K0 with t1. auto. exists t1'. auto. subst. inversion H; subst. exfalso. apply K0 with F1.
+  auto. exists t1'0. auto.
+  inversion H1. exfalso. apply K0 with t2. auto. eauto. exfalso. apply K0 with v1. auto. eauto. apply IHstep in H6.
+  subst. eauto. subst. inversion H1. inversion H3. subst. exfalso. apply K0 with t2. auto. eauto.
+  inversion H0. apply IHstep in H2. subst; auto. subst. inversion H.
+  inversion H0. inversion H1. subst. auto.
+  inversion H0. apply IHstep in H2. subst. auto. subst. inversion H.
+  inversion H0. inversion H1. subst. inversion H0. auto.
+  inversion H0; subst. apply IHstep in H4; subst. auto. exfalso. apply K0 with t1. eauto. eauto.
+  inversion H.
+  inversion H1; subst. exfalso. apply K0 with v1. eauto. eauto.
+  apply IHstep in H6. subst. auto.
+  inversion H0.
+  inversion H0. inversion H3. inversion H4. auto.
+  inversion H0. apply IHstep in H5. subst. auto.
+  subst. inversion H. subst. inversion H. inversion H0. inversion H4. auto. inversion H0. inversion H4. auto.
+  inversion H0. apply IHstep in H4. subst. auto. exfalso. apply K0 with t1. eauto. eauto.
+  inversion H1. exfalso. apply K0 with v1. eauto. eauto. apply IHstep in H6. subst. auto.
+  inversion H0. apply IHstep in H2. subst. auto. subst. inversion H. exfalso. apply K0 with y2. eauto. eauto.
+  exfalso. apply K0 with v2. eauto. eauto. inversion H1. inversion H3. exfalso. apply K0 with v1. eauto. eauto.
+  exfalso. apply K0 with v2. eauto. eauto. auto.
+  inversion H0. apply IHstep in H2. subst. auto. subst. inversion H. exfalso. apply K0 with y2. eauto. eauto.
+  exfalso. apply K0 with v1. eauto. eauto. exfalso. apply K0 with y2. eauto. eauto.
+  inversion H1. inversion H3. exfalso. apply K0 with v1. eauto. eauto.
+  exfalso. apply K0 with v2. eauto. eauto. eauto.
+  inversion H0. apply IHstep in H5. subst. auto. exfalso. apply K0 with t1. eauto. eauto.
+  inversion H0. exfalso. apply K0 with v1. eauto. eauto. auto.
+  inversion H0. apply IHstep in H4. subst. eauto. inversion H0. apply IHstep in H4. subst. eauto.
+  inversion H0. subst. apply IHstep in H7. subst. eauto. subst. inversion H. exfalso. apply K0 with v0. eauto. eauto.
+  subst. inversion H. exfalso. apply K0 with v0. eauto. eauto.
+  inversion H0; subst. inversion H7; subst. exfalso. apply K0 with v0. eauto. eauto. eauto.
+  inversion H0; subst. inversion H7; subst. exfalso. apply K0 with v0. eauto. eauto. auto.
+  inversion H0. apply IHstep in H4. subst; auto. exfalso. apply K0 with t1. eauto. eauto.
+  inversion H1. exfalso. apply K0 with v1. eauto. eauto. apply IHstep in H6. subst; eauto.
+  inversion H0; subst. apply IHstep in H7. subst. auto.
+  inversion H. inversion H. exfalso. apply K0 with v1. eauto. eauto. exfalso. apply K0 with vl. eauto. exists t2'. apply H5. 
+  inversion H0. inversion H6. auto.
+  inversion H1; subst. inversion H8. exfalso. apply K0 with v1. eauto. eauto. exfalso. apply K0 with vl. eauto. exists t2'. apply H6.
+  auto. inversion H0. apply IHstep in H2. subst; eauto. inversion H1. subst. inversion H5. exfalso. apply K0 with F1. eauto. eauto.
+  exfalso. apply K0 with v2. eauto. eauto. auto. }
+
+assert (K2: forall P Q R X, P ==> Q -> Q ==> R -> R ==> P -> P ==>* X -> (X=P \/ X=Q \/ X=R)).
+{ intros. generalize dependent Q. generalize dependent R. induction H2. intros. auto.
+  intros. unfold deterministic in K1. apply K1 with (y2:=Q) in H. subst.
+  assert (z=Q \/ z=R \/ z=x). apply IHmulti. assumption. assumption. assumption. inversion H. auto. inversion H4. auto. auto. auto. }
+unfold not. intros. destruct H. destruct H. inversion K. destruct H1. 
+assert (x=tapp tloop (tnat 0) \/ x=x0 \/ x=x1). inversion H1 as [Q1 [Q2 Q3]]. apply K2; assumption.
+inversion H2. apply H0. exists x0. destruct H1 as [Q1 [Q2 Q3]]. subst. apply Q1.
+inversion H3. subst. apply H0. exists x1. inversion H1 as [Q1 [Q2 Q3]]. apply Q2.
+subst. apply H0. exists (tapp tloop (tnat 0)). inversion H1 as [Q1 [Q2 Q3]]. apply Q3.
+
 Qed.
 
 (*-- Check --*)
